Revert "WIP: Try to change the signature of the Free Monad. Universe problems."
This reverts commit 16e890dd1c6cfe50e28ddc6ee0862f697c7df2bb.

newio/Free.fst
@@ -1,18 +1,27 @@
 module Free
 
 noeq
-type op_sig (op:Type0) = {
+type op_sig (op:Type u#a) = {
   args : op -> Type u#a;
-  res : (cmd:op) -> args cmd -> Type u#b;
+  res : op -> Type u#a;
 }
 
 noeq
-type free (op:Type) (s:op_sig op) (a:Type) : Type =
-| Call : (l:op) -> arg:(s.args l) -> cont:(s.res l arg -> free op s a) -> free op s a
+type free (op:Type0) (s:op_sig op) (a:Type) : Type =
+| Call : (l:op) -> s.args l -> cont:(s.res l -> free op s a) -> free op s a
+| PartialCall : (pre:pure_pre) -> cont:((squash pre) -> free op s a) -> free op s a
 | Return : a -> free op s a
 
 let free_return (op:Type) (s:op_sig op) (a:Type) (x:a) : free op s a =
   Return x
+
+let rec return_of (x:'a) (f:free 'op 's 'a) =
+  match f with
+  | Return x' -> x == x'
+  | Call cmd arg k ->
+     exists r'. return_of x (k r')
+  | PartialCall pre k ->
+     pre ==> return_of x (k ())
 
 let rec free_bind
   (op:Type)
@@ -27,6 +36,9 @@ let rec free_bind
   | Call cmd args fnc ->
       Call cmd args (fun i ->
         free_bind op s a b (fnc i) k)
+  | PartialCall pre fnc ->
+      PartialCall pre (fun _ ->
+        free_bind op s a b (fnc ()) k)
 
 let free_map
   (op:Type)
